mark-and-sweep/impl/GC.Impl.Coalesce.Lemmas.fst
@@ -5,7 +5,6 @@
 module GC.Impl.Coalesce.Lemmas
 
 open FStar.Seq
-open FStar.Mul
 module U64 = FStar.UInt64
 
 open GC.Spec.Base
